SepLogicTime/Transpile.thy
@@ -1,8 +1,13 @@
 theory Transpile
-imports "SepAuto_Time" BinarySearch_Impl DynamicArray2
+imports "SepAuto_Time" 
     "Separation_Logic_Imperative_HOL.Hoare_Triple"  
-  "Refine_Imperative_HOL.Term_Synth" "Monad_Memo_DP.Transform_Cmd"
-  "Refine_Imperative_HOL.Pf_Mono_Prover"
+  "SeprefTime.Term_Synth" "Monad_Memo_DP.Transform_Cmd"
+  "SeprefTime.Pf_Mono_Prover"
+  "SeprefTime.Refine_Automation"
+  keywords  
+    "transpile_define" :: thy_decl and
+    "transpile_replay" :: thy_decl and
+    "transpile_prove" :: thy_decl  
 begin
 
 
@@ -108,11 +113,29 @@ lemma Array_set_conv: "Array_Time.set h a = Array.set h a"
 lemma Array_get_conv: "Array_Time.get h a = Array.get h a"
   unfolding Array_Time.length_def Array.length_def Array.get_def Array_Time.get_def by simp
 
+lemma Array_update_conv: "Array_Time.update a i x h = Array.update  a i x h"
+  unfolding Array_Time.update_def Array.update_def  by (simp add: Array_set_conv Array_get_conv)
+
+lemma Array_alloc_conv: "Array_Time.alloc xs h = Array.alloc xs h"
+  unfolding Array_Time.alloc_def Array.alloc_def Array_set_conv by simp
+
 lemma Array_length_conv: "Array_Time.length h a = Array.length h a"
   unfolding Array_Time.length_def Array.length_def Array_get_conv by simp
 
+
+lemma Ref_set_conv: "Ref_Time.set r x = Ref.set r x"
+  unfolding Ref_Time.set_def Ref.set_def by simp
+
+lemma Ref_get_conv: "Ref_Time.get r x = Ref.get r x"
+  unfolding Ref_Time.get_def Ref.get_def by simp
+
+lemma Ref_alloc_conv: "Ref_Time.alloc x h = Ref.alloc x h"
+  unfolding Ref_Time.alloc_def Ref.alloc_def by (simp add: Ref_set_conv)
+
 subsection \<open>forget\<close>
 
+named_theorems_rev forget_it
+      "Rules for flattening assertions of Imperative-HOL with time"
 
 abbreviation (input) forget :: "(SepAuto_Time.assn) \<Rightarrow> Assertions.assn"
   where "forget P \<equiv> Assertions.Abs_assn (\<lambda>(h,addrs). \<exists>t. (assn_fn (SepAuto_Time.Rep_assn P)) (pHeap h addrs t))"
@@ -145,74 +168,144 @@ lemma assn_fn_models_conv: "assn_fn (SepAuto_Time.assn.Rep_assn A) (pHeap x y t)
       \<longleftrightarrow> (pHeap x y t) \<Turnstile> A"   
   by (simp add: models_def aseval_assn_fn_conv)
 
-lemma forget_it: 
+lemma forget_dollar[forget_it]: 
   "forget ($n) = emp"
-    "forget (A * B) = forget A * forget B"
-  "forget true = true"
-  "forget false = false"
-  "forget (p \<mapsto>\<^sub>a xs) = p \<mapsto>\<^sub>a xs"
-  "forget (q \<mapsto>\<^sub>r v) = q \<mapsto>\<^sub>r v"
-  "forget (\<up>P) = \<up>P"
-  subgoal unfolding timeCredit_assn_def
-    unfolding one_assn_def 
+    unfolding timeCredit_assn_def
+    unfolding one_assn_def  
      apply(subst   SepAuto_Time.Abs_assn_inverse   )
     subgoal apply auto
       unfolding SepAuto_Time.proper_def by auto 
     apply(rule arg_cong[where f=Assertions.assn.Abs_assn])
     apply(rule ext) by auto 
-  subgoal 
-    apply (rule  ) apply rule
-    subgoal for h unfolding mod_star_conv
-      apply auto unfolding assn_fn_models_conv
-      apply(drule SepAuto_Time.mod_star_convE) apply auto
-      subgoal  for x as1 as2 n1 n2
-        apply(rule exI[where x=as1])
-        apply(rule exI[where x=as2]) apply auto
-        subgoal                           
-          apply(subst   Abs_assn_inverse  )
-          subgoal apply (auto simp: Assertions.proper_def)
-            subgoal  
-              using Assertions.in_range.simps SepAuto_Time.models_in_range by auto  
-            subgoal  
-              using SepAuto_Time.mod_relH relH_eq by fastforce   
-            done
-          apply simp apply(rule exI[where x=n1]) by simp
-        subgoal                           
-          apply(subst   Abs_assn_inverse  )
-          subgoal apply (auto simp: Assertions.proper_def)
-            subgoal  
-              using Assertions.in_range.simps SepAuto_Time.models_in_range by auto  
-            subgoal  
-              using SepAuto_Time.mod_relH relH_eq by fastforce   
-            done
-          apply simp apply(rule exI[where x=n2]) by simp
-        done
-      done
-    subgoal for h unfolding mod_star_conv assn_fn_models_conv
-      apply auto
-          apply(subst  (asm) Abs_assn_inverse  )
-      subgoal apply (auto simp: Assertions.proper_def)
-            subgoal  
-              using Assertions.in_range.simps SepAuto_Time.models_in_range by auto  
-            subgoal  
-              using SepAuto_Time.mod_relH relH_eq by fastforce   
-            done
-          apply(subst  (asm) Abs_assn_inverse  )
-      subgoal apply (auto simp: Assertions.proper_def)
-            subgoal  
-              using Assertions.in_range.simps SepAuto_Time.models_in_range by auto  
-            subgoal  
-              using SepAuto_Time.mod_relH relH_eq by fastforce   
-            done
-          apply auto
-          subgoal for hr as1 as2 t ta
-            apply(rule exI[where x="t+ta"])
-            apply(rule SepAuto_Time.mod_star_convI)
-            by auto
-          done
-        done
-      sorry
 
+lemma  forget_star[forget_it]:
+  "forget (A * B) = forget A * forget B"
+  apply (rule  ) apply rule
+  subgoal for h unfolding mod_star_conv
+    apply safe
+    unfolding assn_fn_models_conv
+    apply(drule SepAuto_Time.mod_star_convE)
+    apply auto
+    subgoal  for x as1 as2 n1 n2
+      apply(rule exI[where x=as1])
+      apply(rule exI[where x=as2]) apply auto
+      subgoal                           
+        apply(subst   Abs_assn_inverse  )
+        subgoal apply (auto simp: Assertions.proper_def)
+          subgoal  
+            using Assertions.in_range.simps SepAuto_Time.models_in_range by auto  
+          subgoal  
+            using SepAuto_Time.mod_relH relH_eq by fastforce   
+          done
+        apply simp apply(rule exI[where x=n1]) by simp
+      subgoal                           
+        apply(subst   Abs_assn_inverse  )
+        subgoal apply (auto simp: Assertions.proper_def)
+          subgoal  
+            using Assertions.in_range.simps SepAuto_Time.models_in_range by auto  
+          subgoal  
+            using SepAuto_Time.mod_relH relH_eq by fastforce   
+          done
+        apply simp apply(rule exI[where x=n2]) by simp
+      done
+    done
+  subgoal for h unfolding mod_star_conv assn_fn_models_conv 
+    apply(subst  (asm) Abs_assn_inverse  )
+    subgoal apply (auto simp: Assertions.proper_def)
+      subgoal  
+        using Assertions.in_range.simps SepAuto_Time.models_in_range by auto  
+      subgoal  
+        using SepAuto_Time.mod_relH relH_eq by fastforce   
+      done
+    apply(subst  (asm) Abs_assn_inverse  )
+    subgoal apply (auto simp: Assertions.proper_def)
+      subgoal  
+        using Assertions.in_range.simps SepAuto_Time.models_in_range by auto  
+      subgoal  
+        using SepAuto_Time.mod_relH relH_eq by fastforce   
+      done
+    apply auto
+    subgoal for hr as1 as2 t ta
+      apply(rule exI[where x="t+ta"])
+      apply(rule SepAuto_Time.mod_star_convI)
+      by auto
+    done
+  done
+
+lemma forget_other[forget_it]:
+  "forget true = true"
+  "forget (\<up>P) = \<up>P"
+  "forget false = false"
+  "forget (p \<mapsto>\<^sub>a xs) = p \<mapsto>\<^sub>a xs"
+  "forget (q \<mapsto>\<^sub>r v) = q \<mapsto>\<^sub>r v"
+  subgoal   
+    apply rule
+    apply rule
+    subgoal for h  
+      using Assertions.in_range.simps assn_fn_models_conv top_assn_rule by auto  
+    subgoal for h
+      apply safe
+      apply(rule exI[where x=0])       
+      by (simp add: Assertions.in_range.simps assn_fn_models_conv top_assn_rule) 
+    done
+  subgoal 
+    by(auto intro: Abs_assn_eqI
+            simp: SepAuto_Time.pure_assn_def SepAuto_Time.Abs_assn_inverse
+                  SepAuto_Time.proper_def )
+  subgoal 
+    by(auto intro: Abs_assn_eqI
+            simp: SepAuto_Time.pure_assn_def SepAuto_Time.Abs_assn_inverse
+                  SepAuto_Time.proper_def )
+  subgoal apply(rule)
+    apply rule 
+    subgoal for h unfolding SepAuto_Time.snga_assn_def Assertions.snga_assn_def 
+      apply(subst (asm)  SepAuto_Time.Abs_assn_inverse   )
+      subgoal by(auto simp: SepAuto_Time.proper_def  SepAuto_Time.relH_array)  
+      subgoal by (auto simp add: Array_get_conv Assertions.assn.Abs_assn_inverse) 
+      done
+    subgoal for h  unfolding SepAuto_Time.snga_assn_def Assertions.snga_assn_def
+      apply(subst  SepAuto_Time.Abs_assn_inverse   )
+      subgoal by(auto simp: SepAuto_Time.proper_def SepAuto_Time.relH_array) 
+      subgoal by (auto simp add: Array_get_conv Assertions.assn.Abs_assn_inverse) 
+      done
+    done
+  subgoal apply(rule)
+    apply rule 
+    subgoal for h unfolding SepAuto_Time.sngr_assn_def Assertions.sngr_assn_def 
+      apply(subst (asm)  SepAuto_Time.Abs_assn_inverse   )
+      subgoal by(auto simp: SepAuto_Time.proper_def  SepAuto_Time.relH_ref)  
+      subgoal by (auto simp add: Ref_get_conv Assertions.assn.Abs_assn_inverse) 
+      done
+    subgoal for h  unfolding SepAuto_Time.sngr_assn_def Assertions.sngr_assn_def 
+      apply(subst  SepAuto_Time.Abs_assn_inverse   )
+      subgoal by(auto simp: SepAuto_Time.proper_def SepAuto_Time.relH_ref) 
+      subgoal by (auto simp add: Ref_get_conv Assertions.assn.Abs_assn_inverse) 
+      done
+    done
+  done
+
+
+lemma forget_ex[forget_it]: "forget (\<exists>\<^sub>A x. P x) = (\<exists>\<^sub>A x. forget (P x))"
+  apply rule
+  apply rule
+  subgoal for h apply safe
+    unfolding SepAuto_Time.ex_assn_def 
+      apply(subst (asm)  SepAuto_Time.Abs_assn_inverse   )
+    subgoal using SepAuto_Time.models_in_range 
+        apply (auto simp: SepAuto_Time.proper_def  ) 
+      using SepAuto_Time.mod_relH by blast
+    apply auto  
+    using modelsT_forget_models by blast  
+  subgoal for h apply safe
+    unfolding SepAuto_Time.ex_assn_def 
+      apply(subst   SepAuto_Time.Abs_assn_inverse   )
+    subgoal using SepAuto_Time.models_in_range 
+        apply (auto simp: SepAuto_Time.proper_def  ) 
+      using SepAuto_Time.mod_relH by blast
+    apply auto   
+    using models_forget_modelsT by blast  
+  done
+ 
 
 subsection \<open>flatten\<close>
 
@@ -359,12 +452,15 @@ lemma refines_HT: assumes "refines c' c" and "SepAuto_Time.hoare_triple P c Q"
 
 
 
+named_theorems_rev transpile_rules
+      "Rules for transpiling from Imperative-HOL with time
+        to vanilla Imperative-HOL"
 
 subsubsection \<open>refines for combinators\<close>
 
 lemma refines_combinators: 
   "refines m' m \<Longrightarrow> (\<And>v. refines (f' v) (f v)) \<Longrightarrow> refines (m' \<bind> f') (m \<bind> f)"
-    "refines x' x \<Longrightarrow> refines y' y \<Longrightarrow> refines (if b then x' else y') (if b then x else y)"
+    "(b \<Longrightarrow> refines x' x) \<Longrightarrow> (~b \<Longrightarrow> refines y' y) \<Longrightarrow> refines (if b then x' else y') (if b then x else y)"
   "refines (return v) (Heap_Time_Monad.return v)"
   "refines (F' n) (F n) \<Longrightarrow> refines (Let n F') (Let n F)" 
   subgoal 
@@ -397,7 +493,83 @@ lemma refines_combinators:
   subgoal unfolding refines_def by auto
   done 
 
+lemma [transpile_rules]:   "
+  (\<And>a b. refines (f' a b) (f a b)) \<Longrightarrow>
+  refines (case x of (a,b) \<Rightarrow> f' a b) (case x of (a,b) \<Rightarrow> f a b)"
+  by (auto split: prod.splits)
+
+lemma [transpile_rules]:   "refines (return v) (ureturn v)"
+  unfolding refines_def return_def ureturn_def
+    Heap_Time_Monad.effect_def Heap_Monad.effect_def
+    Heap_Time_Monad.heap_def Heap_Monad.heap_def
+  by auto
+
+lemma [transpile_rules]: "refines f' f 
+  \<Longrightarrow> (\<And>y. refines (g' y) (g y)) \<Longrightarrow> 
+refines (case x of None \<Rightarrow> f' | Some y \<Rightarrow> g' y)  (case x of None \<Rightarrow> f | Some y \<Rightarrow> g y)"
+  by (auto split: option.splits)
+
+lemma assumes  M: "(\<And>x. Heap_Time_Monad.mono_Heap (\<lambda>f. F f x))" 
+    and M2: "\<And>x. Heap_Monad.mono_Heap (\<lambda>f. F' f x)"
+and S: "(\<And>f f' x h h' r n.
+    (\<And>x h h' r n. Heap_Time_Monad.effect (f x) h h' r n \<Longrightarrow> Heap_Monad.effect (f' x) h h' r) \<Longrightarrow>
+    Heap_Time_Monad.effect (F f x) h h' r n \<Longrightarrow> Heap_Monad.effect (F' f' x) h h' r)"
+shows effect_fixp:
+"\<And>h h' r n x. Heap_Time_Monad.effect (Heap_Time_Monad.heap.fixp_fun F x) h h' r n \<Longrightarrow> Heap_Monad.effect (Heap_Monad.heap.fixp_fun F' x) h h' r"
+  apply(rule Heap_Time_Monad.fixp_induct_heap[where U=id and C=id and F=F, simplified,
+        where P="\<lambda>x h h' r n. Heap_Monad.effect (Heap_Monad.heap.fixp_fun F' x) h h' r", simplified])
+
+  subgoal apply(rule M ) done
+    apply simp defer
+   apply simp
+
+  apply (subst heap.mono_body_fixp[OF M2] ) 
+  apply(rule S[where f'="(Heap_Monad.heap.fixp_fun F')"])
+   apply blast
+  apply blast
+  done
+
+lemma refines_fixp[transpile_rules]:
+  assumes M: "(\<And>x. Heap_Time_Monad.mono_Heap (\<lambda>f. F f x))" 
+  assumes  S: "(\<And>f f' x h h' r n.
+         (\<And>x. refines (f' x) (f x) ) \<Longrightarrow> refines (F' f' x) (F f x) )"
+  assumes M2: "\<And>x. Heap_Monad.mono_Heap (\<lambda>f. F' f x)"
+  shows "\<And>h h' r n x. refines
+    (Heap_Monad.heap.fixp_fun F' x) (Heap_Time_Monad.heap.fixp_fun F x)"
+  using S unfolding refines_def apply safe apply(rule effect_fixp[OF M M2]) by blast+  
+
+
+
+
 subsubsection \<open>Refines for basic operations\<close>
+
+
+
+
+lemma refines_ref_lookup[transpile_rules]: "refines (Ref.lookup r) (Ref_Time.lookup r)"
+  unfolding refines_def Heap_Time_Monad.effect_def Heap_Monad.effect_def
+        Ref_Time.lookup_def Ref.lookup_def
+        Heap_Time_Monad.tap_def Heap_Monad.tap_def
+        Heap_Time_Monad.heap_def Heap_Monad.heap_def
+  by (auto simp: Ref_get_conv )
+
+lemma refines_ref[transpile_rules]: "refines (Ref.ref x) (Ref_Time.ref x)"
+  unfolding refines_def Heap_Time_Monad.effect_def Heap_Monad.effect_def
+        Ref_Time.ref_def Ref.ref_def
+        Heap_Time_Monad.heap_def Heap_Monad.heap_def
+  by (auto simp: Ref_alloc_conv split: prod.splits)
+
+lemma refines_ref_update[transpile_rules]: "refines (Ref.update r v) (Ref_Time.update r v)"
+  unfolding refines_def Heap_Time_Monad.effect_def Heap_Monad.effect_def
+        Ref_Time.update_def Ref.update_def
+        Heap_Time_Monad.heap_def Heap_Monad.heap_def
+  by (auto simp: Ref_set_conv )
+
+lemma refines_raise[transpile_rules]:
+  "refines (Heap_Monad.raise (String.implode msg)) (Heap_Time_Monad.raise msg)"
+  unfolding refines_def Heap_Time_Monad.effect_def Heap_Monad.effect_def
+        Heap_Time_Monad.raise_def Heap_Monad.raise_def
+  by auto
 
 lemma refines_nth:
     "refines (Array.nth a l) (Array_Time.nth a l)"
@@ -407,62 +579,758 @@ lemma refines_nth:
     by (auto simp: Array_length_conv Array_get_conv)
 
 
-named_theorems_rev transpile_rules
-      "Rules for transpiling from Imperative-HOL with time
-        to vanilla Imperative-HOL"
+lemma refines_freeze:
+    "refines (Array.freeze a) (Array_Time.freeze a)"
+  unfolding refines_def Heap_Time_Monad.effect_def Heap_Monad.effect_def
+          Array_Time.freeze_def  Array.freeze_def  
+        Heap_Time_Monad.heap_def Heap_Monad.heap_def
+          Heap_Time_Monad.tap_def  Heap_Monad.tap_def
+  by (auto simp: Array_length_conv Array_get_conv)
 
 
-lemmas [transpile_rules] = refines_combinators refines_nth
+lemma refines_of_list:
+    "refines (Array.of_list xs) (Array_Time.of_list xs)"
+  unfolding refines_def Heap_Time_Monad.effect_def Heap_Monad.effect_def
+          Array_Time.of_list_def  Array.of_list_def  
+        Heap_Time_Monad.heap_def Heap_Monad.heap_def
+          Heap_Time_Monad.tap_def  Heap_Monad.tap_def
+  apply (auto simp: Array_length_conv Array_alloc_conv split: option.splits)  
+  by (smt Array.alloc_def fst_conv prod.case_eq_if snd_conv)  
+ 
 
-section \<open>Transpilation by hand -- an example\<close>
+lemma refines_array_upd:
+    "refines (Array.upd i x a) (Array_Time.upd i x a)"
+  unfolding refines_def Heap_Time_Monad.effect_def Heap_Monad.effect_def
+          Array_Time.upd_def  Array.upd_def 
+          Heap_Time_Monad.guard_def  Heap_Monad.guard_def
+  by (auto simp: Array_length_conv Array_update_conv)
 
-schematic_goal p: "refines ?G (binarysearch l r x a)"   
-  apply(subst binarysearch.simps)
-  apply(rule transpile_rules refines_flatten)+ done
+lemma refines_array_new:
+    "refines (Array.new n x) (Array_Time.new n x)"
+  unfolding refines_def Heap_Time_Monad.effect_def Heap_Monad.effect_def
+          Array_Time.new_def  Array.new_def 
+          Heap_Time_Monad.guard_def  Heap_Monad.guard_def
+        Heap_Time_Monad.heap_def Heap_Monad.heap_def
+  apply (auto simp: Array_length_conv Array_alloc_conv split: option.splits)  
+  by (smt Array.alloc_def fst_conv prod.case_eq_if snd_conv)  
 
-partial_function (heap) aahh where
-"aahh l r x a = (if r \<le> l then Heap_Monad.return False
-  else if r \<le> l + 1 then Array.nth a l \<bind> (\<lambda>v. Heap_Monad.return (v = x))
-       else let b = avg l r
-            in Array.nth a b \<bind>
-               (\<lambda>c. if c = x then Heap_Monad.return True
-                    else if c < x then aahh (b + 1) r x a else aahh l b x a))"
 
-lemma refines_binarysearch: "refines (aahh l r x a) (binarysearch l r x a)"
-  unfolding refines_def
-proof safe
-  fix h h' ra n
-  assume *: "Heap_Time_Monad.effect (binarysearch l r x a) h h' ra n"
+lemma refines_len:
+    "refines (Array.len a) (Array_Time.len a)"
+  unfolding refines_def Heap_Time_Monad.effect_def Heap_Monad.effect_def
+          Array_Time.len_def  Array.len_def 
+          Heap_Time_Monad.tap_def  Heap_Monad.tap_def
+  by (auto simp: Array_length_conv)
+
+
+
+lemmas [transpile_rules] = refines_combinators
+  refines_nth refines_len refines_array_upd refines_array_new
+  refines_freeze refines_of_list
+
+
+section \<open>Automating Transpilation\<close>
+
+
+ML \<open>                      
+
+
+    fun myprint_tac' ctxt  st = 
+      let val _ = tracing ("..>");
+          val _ = tracing (Thm.string_of_thm ctxt st)
+      in all_tac st end
+
+    fun myprint_tac ctxt str _ st = 
+      let val _ = tracing ("..> " ^str);
+          val _ = tracing (Thm.string_of_thm ctxt st)
+      in all_tac st end
+
+
+
+    fun dest_hol_flatten_eq_prop t =
+      let
+        val Const ("HOL.Trueprop", _) $ (Const ("HOL.eq", _) $ a $ b) = t
+        val (Const ("Experiment.flatten", _) $ c) = a
+      in (c, b) end
+   fun split_off_typ (Type("fun",[S,T])) = 
+              (case split_off_typ T of (L,Hd) => (S::L, Hd))
+        | split_off_typ t = ([],t) 
+
+      fun close_fun co ctxt = let   
+        val co_ty = Term.type_of co
+        val (es,e) = split_off_typ co_ty
+        val nctxt = Variable.names_of ctxt    
+        val vars = Name.invent nctxt "" (length es) 
+        val vars = map Free (vars ~~ es)
+        in
+          (vars, fold (fn v => fn f => f $ v) vars co)
+      end
+
+      fun close_fun_schem co ctxt = let   
+        val co_ty = Term.type_of co
+        val (es,e) = split_off_typ co_ty
+        val nctxt = Variable.names_of ctxt    
+        val vars = Name.invent nctxt "" (length es) 
+        val vars = map Var ((map (fn x => (x,0)) vars) ~~ es)
+        in
+          (vars, fold (fn v => fn f => f $ v) vars co)
+      end
+
+    fun add_partial_function bind def_eq =
+      let
+        val fixes = [(bind, NONE, NoSyn)];
+        val specs = (fn def => ((Binding.empty, @{attributes [code]}), def)) def_eq
+        val str = "heap"
+      in
+        Partial_Function.add_partial_function str fixes specs 
+    end
+
+    fun add_function bind defs =
+      let
+        val fixes = [(bind, NONE, NoSyn)];
+        val specs = map (fn def => (((Binding.empty, []), def), [], [])) defs
+        val pat_completeness_auto = fn ctxt =>
+          Pat_Completeness.pat_completeness_tac ctxt 1
+          THEN auto_tac ctxt
+      in
+        Function.add_function fixes specs Function_Fun.fun_config pat_completeness_auto
+    end
+
+    fun split_off_typ (Type("fun",[S,T])) = 
+              (case split_off_typ T of (L,Hd) => (S::L, Hd))
+        | split_off_typ t = ([],t)
+    fun comb_typ (x::xs,Hd) = (Type("fun",[x,comb_typ (xs,Hd)])) 
+        | comb_typ ([],Hd) = Hd
   
-  note f =  binarysearch.raw_induct[where P="\<lambda>l r x a h h' ra n. Heap_Monad.effect (aahh l r x a) h h' ra", where xa="(((l,r),x),a)", simplified]
 
-  show "Heap_Monad.effect (aahh l r x a) h h' ra" 
-  proof (rule f[OF _ *], goal_cases) 
-    case (1 f l r x a la ra xa aa)
-    from 1(1) have IH: "\<And>l r x a. refines (aahh l r x a) (f l r x a) " unfolding refines_def by auto 
-    show ?case apply(rule refinesD1[OF _ 1(2)])
-      apply(subst aahh.simps)
-      apply(rule transpile_rules IH)+
-      done
-  qed
-qed
-
-thm refines_HT'[OF _ refines_binarysearch]
+fun defined_by_partial_function ctxt t =
+  (case t of Const (f_str, _) =>
+      (length ( Proof_Context.get_thms ctxt (f_str^".raw_induct")) > 0)
+               handle error => false
+      | _ => false)
 
 
-lemma flatten_correct: "sorted xs \<Longrightarrow> r \<le> length xs \<Longrightarrow> l \<le> r \<Longrightarrow>
-   <a \<mapsto>\<^sub>a xs > aahh l r x a
-       <\<lambda>ra. a \<mapsto>\<^sub>a xs * \<up> (ra = (\<exists>i\<ge>l. i < r \<and> xs ! i = x))>\<^sub>t"
-  apply(rule refines_HT) 
-     apply(rule refines_binarysearch)
-    apply(rule binarysearch_correct')
-      apply simp
-     apply simp
-    apply simp
-   apply (simp add: forget_it)
-  apply(rule ext) apply (simp add: forget_it)
-  done 
 
+fun mono_side_tac ctxt = Subgoal.FOCUS_PARAMS (fn {context = ctxt, ...} => ALLGOALS (
+      SUBGOAL (fn (t, _) => case Logic.strip_imp_concl t of
+        @{mpat "Trueprop (Heap_Time_Monad.mono_Heap ?a)"} => 
+          Pf_Mono_Prover.mono_tac ctxt 1
+       | 
+        @{mpat "Trueprop (Heap_Monad.mono_Heap ?a)"} => 
+          Pf_Mono_Prover.mono_tac ctxt 1
+       |  _ => no_tac
+      ))
+    ) ctxt 
+
+fun mkk binding def_thms termination ctxt =
+  let 
+
+
+    val fun_def = def_thms
+
+    val eqns = map Thm.concl_of  def_thms
+    val (eqns, _) = Variable.import_terms true eqns ctxt
+
+    fun dest_hol_refines_prop t =
+      let
+        val Const ("HOL.Trueprop", _) $ (Const ("Transpile.refines", _) $ a $ b) = t
+      in (a, b) end
+    fun dest_hol_eq_prop t =
+      let
+        val Const ("HOL.Trueprop", _) $ (Const ("HOL.eq", _) $ a $ b) = t
+      in (a, b) end
+    fun get_fun_term_head t =
+      let
+        val (t, _) = dest_hol_eq_prop t
+        val t = Term.head_of t
+     in t end
+    fun get_fun_head t =
+      let
+        val (t, _) = dest_hol_flatten_eq_prop t
+        val t = Term.head_of t
+        val Const (fun_name, fun_ty) = t
+     in (fun_name, fun_ty) end
+   
+  val _ = tracing "here"
+
+
+    val (old_info, part_f)  = let
+          val (lhs, rhs) = dest_hol_eq_prop (hd eqns)
+          val (f, args) = Term.strip_comb lhs
+          val old_info = Function_Common.import_function_data f ctxt  
+          val flag = defined_by_partial_function ctxt f
+      in
+          (old_info, flag)
+      end
+
+    val _ = (case old_info of NONE => tracing ("not defined via the function package!")
+                | SOME old_info => tracing "defined via the function package!")
+
+
+      (* for a defining equation synthesize a flattened equation theorem *)                            
+      fun synthesize2 ctxt def_thm =
+        let 
+          val ctxt_orig = ctxt
+          val fun_def = def_thm
+
+          val eqn = Thm.concl_of def_thm
+
+          val (lhs, rhs) = dest_hol_eq_prop eqn
+          val (f, args) = Term.strip_comb lhs
+ 
+          val t = @{mk_term "?lhs"} 
+          val t_goal = @{mk_term "flatten ?lhs"} 
+
+   
+          val ([t,t_goal,eqn], ctxt) = (Variable.import_terms true) [t,t_goal,eqn] ctxt 
+          val ty = Term.type_of t 
+          val t_goaly = Term.type_of t_goal
+          val  _ = tracing ("bra")
+
+
+          val v = Var (("result",0), t_goaly)
+          val  _ = tracing ("ff")
+          val  _ = tracing ("t " ^ Syntax.string_of_term ctxt t)
+          val  _ = tracing ("ty " ^ Syntax.string_of_typ ctxt ty)
+          val goal = @{mk_term "Trueprop (refines ?v ?t)"} |> Thm.cterm_of ctxt
+          val  _ = tracing ("goal " ^ Syntax.string_of_term ctxt @{mk_term "Trueprop (refines ?v ?t)"})
+    
+
+          val  _ = tracing ("fnn")
+          val transpile_rules =  (Named_Theorems_Rev.get ctxt @{named_theorems_rev transpile_rules})
+
+
+
+          val flatten_rules =  ( transpile_rules @ [@{thm refines_flatten}] ) |> Tactic.build_net
+          val _ = EqSubst.eqsubst_tac
+          fun tac ctxt =  (ALLGOALS ((EqSubst.eqsubst_tac ctxt [0] [fun_def]  )
+                  THEN' (TRY_SOLVED' (REPEAT_DETERM' (CHANGED o 
+                      FIRST' [ resolve_from_net_tac ctxt flatten_rules,
+                                Method.assm_tac ctxt,
+                                mono_side_tac ctxt ])))))
+
+          (* synthesize by using flatten rules *)
+          val thm = Goal.prove_internal ctxt [] goal (fn _ => tac ctxt)
+
+          val  _ = tracing ("proof successfull")
+        
+        in
+          singleton (Variable.export ctxt ctxt_orig) thm
+        end  
+
+    val flat_thms = map (synthesize2 ctxt) def_thms
+
+  val _ = tracing "here2"
+    (* give the theorem a name *)
+    val (_, ctxt) = Local_Theory.note (
+      (Binding.qualify_name true binding "flattens", []),
+      flat_thms
+    ) ctxt  
+
+    val thm = hd flat_thms
+
+    val s = Binding.name_of binding
+      
+    
+    fun prepare_equation ctxt (def_thm, flat_thm) =
+      let 
+        val ctxt_orig = ctxt
+        val  _ = tracing ("prepare_equation")
+        val (f_name, f_ty) = let
+            val eqn = Thm.concl_of def_thm
+            val (eqn, ctxt1) = yield_singleton (Variable.import_terms true) eqn ctxt
+            val (lhs, rhs) = dest_hol_eq_prop eqn
+            val (f, _) = Term.strip_comb lhs
+            val Const (f_name, f_ty) = f
+          in 
+            (f_name, f_ty)
+          end
+        val orig_head = Const (f_name, f_ty)
+
+        val fl_eqn = Thm.concl_of flat_thm
+        val  _ = tracing ("before " ^ Syntax.string_of_term ctxt fl_eqn)
+        val (fl_eqn, ctxt1) = yield_singleton (Variable.import_terms true) fl_eqn ctxt
+        val _ = tracing ("after " ^ Syntax.string_of_term ctxt1 fl_eqn)
+        val _ = Specification.read_multi_specs
+        fun my_replace t v = let
+          val  _ = tracing "start my_replace"
+          fun r (t1$t2) =  
+              let
+                val found = (case t1 of (Const ("Transpile.flatten", _))
+                  => let
+                      val hot2 = Term.head_of t2 
+                      val _ = tracing (Syntax.string_of_term ctxt1 hot2)
+                     in (case hot2 of (Const (f_name, _)) =>
+                                (* replace *)
+                             let val (f,fs) = strip_comb t2
+                                     in 
+                              (if f <> orig_head then error ("Missing flatten rule for " ^ Syntax.string_of_term ctxt f) else
+                           SOME (list_comb (v,fs))   ) end
+                           | _ => NONE)
+                     end
+                  | _ =>   NONE)
+                in (case found of SOME t' => t'
+                     | NONE => r t1  $ r t2 )
+              end
+            | r (Abs (x,T,t))  =
+                let val t = r t 
+                in (Abs (x,T,t)) end
+            | r t = t
+          in r t
+          end 
+
+        val  _ = tracing ("split " ^ Syntax.string_of_term ctxt fl_eqn)
+        val (rhs,lhs) = dest_hol_refines_prop fl_eqn
+        val lhs = @{mk_term "flatten ?lhs"}
+        val (es,e) = split_off_typ f_ty
+        val ee = comb_typ (es, Term.type_of lhs)
+        val vv =   Free (s, ee) 
+
+        val R = my_replace lhs vv  
+        val RR = my_replace rhs vv   
+        
+        val _ = tracing (Syntax.string_of_term ctxt R)
+        val _ = tracing (Syntax.string_of_term ctxt RR)
+        val feq = @{mk_term "Trueprop (?R = ?RR)"} 
+     (*   val feq = singleton  (Variable.export_terms ctxt1 ctxt_orig) feq *)
+      in  feq end
+ 
+
+    val feq2 = map (prepare_equation ctxt) (def_thms ~~ flat_thms)
+ 
+    val _ = tracing "defining equations:"
+    val _ = map (fn x => tracing (Syntax.string_of_term ctxt x)) feq2
+    val _ = tracing "aha"
+ 
+
+
+
+    val ctxt = (case old_info of NONE =>
+            let
+              val _ =  tracing ("not defined via the function package!")
+              val [feq2] = feq2
+              val ctxt = (if part_f
+                  then let 
+                    val ((t, _), ctxt) = add_partial_function binding feq2 ctxt
+                  in ctxt end
+                  else let
+                    val _ = tracing "normal definition, not recursive!" 
+                    
+                    val ((_,(_,def_thm)),ctxt) =
+                           Specification.definition 
+                                    (SOME (binding,NONE,Mixfix.NoSyn)) [] []
+                                     ((Binding.empty,@{attributes [code]}),feq2) ctxt
+                    in ctxt end )
+          in ctxt end
+                | SOME old_info =>
+            let
+            val _ =  tracing "defined via the function package!"
+            val (new_info, ctxt) = add_function binding feq2 ctxt
+            in ctxt
+            end )
+ 
+
+   val _ = tracing "oha"
+  in
+    (ctxt )
+  end
+
+fun transpile_define_cmd ((termination, binding), thm_refs) lthy =
+  let
+    val def_thms = Attrib.eval_thms lthy thm_refs
+  val _ = tracing "transpile_define"
+  val  ctxt  = mkk binding def_thms (termination <> NONE) lthy
+  in
+      ctxt
+  end
+
+val transpile_define_parser =
+  Scan.option (Parse.$$$ "(" |-- Parse.reserved "prove_termination" --| Parse.$$$ ")")
+  -- (Parse.binding --| Parse.$$$ ":") (* scope, e.g., bf\<^sub>T *)
+  -- Parse.thms1
+
+val _ =
+  Outer_Syntax.local_theory @{command_keyword transpile_define}
+  "Transpile from Imperative-HOL with time to vanilla Imperative-HOL, stripping away time counting"
+    (transpile_define_parser >> transpile_define_cmd)
+
+
+fun transpile_replay_cmd  (t_new, t_old) ctxt =
+  let
+    val t_new = Syntax.read_term ctxt t_new;
+    val SOME new_info = Function_Common.import_function_data t_new ctxt
+    val t_old = Syntax.read_term ctxt t_old;
+    val old_info = Function_Common.import_function_data t_old ctxt
+    
+  fun totality_replay_tac old_info new_info ctxt =
+    let
+      val totality0 = Transform_Misc.totality_of old_info
+      val def0 = Transform_Misc.rel_of old_info ctxt
+    val _ = tracing ("AA") 
+  val _ = tracing (Thm.string_of_thm ctxt def0) 
+      val def1 = Transform_Misc.rel_of new_info ctxt
+  val _ = tracing (Thm.string_of_thm ctxt def1) 
+      fun my_print_tac msg st = (tracing msg; all_tac st)
+    in  (Transform_Tactic.totality_resolve_tac totality0 def0 def1 ctxt
+        THEN my_print_tac "termination by replaying") 
+    end
+ 
+    val lthy = ctxt
+
+    val replay_tac = case old_info of
+      NONE => no_tac
+    | SOME info => 
+      myprint_tac' ctxt THEN totality_replay_tac info new_info lthy
+    val totality_tac =
+      myprint_tac' ctxt THEN
+      ((
+      myprint_tac' ctxt THEN replay_tac)
+      ORELSE (Function_Common.termination_prover_tac false lthy
+        THEN Transform_Tactic.my_print_tac "termination by default prover"))
+
+    val (_, ctxt) = Function.prove_termination NONE replay_tac lthy
+ 
+    val _ = tracing "fff_cmd"
+  in
+    ctxt
+end
+
+val transpile_replay_parser =
+   Parse.term  --
+   Parse.term 
+ 
+val _ =
+  Outer_Syntax.local_theory @{command_keyword transpile_replay}
+  "Define a new ground constant from an existing function definition"
+    (transpile_replay_parser >> transpile_replay_cmd)
+\<close>
+
+
+
+subsection \<open>transpile_prove\<close>
+
+lemma ff1: "a=a' \<Longrightarrow> b=b' \<Longrightarrow> Heap_Monad.bind a b =  Heap_Monad.bind a' b'"
+  by auto
+lemma ff: "a=a' \<Longrightarrow> (\<And>x. b x = b' x) \<Longrightarrow> Heap_Monad.bind a b =  Heap_Monad.bind a' b'"
+  apply(rule ff1) apply simp apply (rule ext) by simp
+
+lemma rr: "\<And>aa. (aa \<Longrightarrow> b=b') \<Longrightarrow> (~aa\<Longrightarrow> c=c') \<Longrightarrow> (if aa then b else c) = (if aa then b' else c')"
+  apply auto done
+
+
+ML\<open>
+
+fun mkk2 t t2 ctxt =
+  let 
+    val transpile_rules =  (Named_Theorems_Rev.get ctxt @{named_theorems_rev transpile_rules})
+
+    fun split_off_typ (Type("fun",[S,T])) = 
+              (case split_off_typ T of (L,Hd) => (S::L, Hd))
+        | split_off_typ t = ([],t)
+    val _ = tracing "mkk2"    
+  
+    val te = Syntax.read_term ctxt t;
+    val (varsb,psc) = close_fun_schem te ctxt  
+
+    val te2 = Syntax.read_term ctxt t2;
+    val (varsb,ppsc) = close_fun_schem te2 ctxt 
+
+    val goal_t = @{mk_term "Trueprop (refines ?psc ?ppsc)"} 
+
+    val old_info  = Function_Common.import_function_data te ctxt   
+
+    val _ = (case old_info of NONE => tracing (Syntax.string_of_term ctxt te
+                                           ^ " was defined via the partial function package")
+            | SOME old_info => tracing (Syntax.string_of_term ctxt te
+                                           ^ " was defined via the function package"))  
+
+    fun via_part_fun te te2 varsb = let
+      fun mk_effect ctxt psc =
+        let  
+          val ef = @{mk_term "effect ?psc"}
+          val (_, ctxt) = yield_singleton (Variable.import_terms true) ef ctxt
+          val (vc, p) = close_fun_schem ef ctxt   
+          val (_, ctxt) = yield_singleton (Variable.import_terms true) p ctxt
+          
+          val nctxt = Variable.names_of ctxt    
+          val vars = Name.invent nctxt "" 1 
+          val vars_n = map Var ((map (fn x => (x,0)) vars) ~~ [natT])
+          
+          val _ = tracing ("AA "  ^ (Syntax.string_of_term ctxt p))
+          val tea = fold_rev lambda (varsb @ vc @ vars_n ) p
+          val _ = tracing ("C "  ^ (Syntax.string_of_term ctxt tea))
+        in tea end
+
+      val insta = mk_effect ctxt psc
+      val _ = tracing ("INSTA"  ^ (Syntax.string_of_term ctxt insta))
+  
+      
+  
+      (* try to prove the goal *)
+      fun prove_goal ctxt goal =
+        let
+          val ctxt_orig = ctxt
+          val (goal :: varsb, ctxt) =  Variable.import_terms true (goal :: varsb) ctxt
+          val _ = tracing (Syntax.string_of_term ctxt goal)
+          val Const ("HOL.Trueprop", _) $ goal_t_bool = goal 
+          val goal_t = goal 
+          val _ = tracing ("GoAL:"^Syntax.string_of_term ctxt goal_t)
+          val goal = goal |> Thm.cterm_of ctxt  
+  
+          val my_ss = put_simpset HOL_basic_ss ctxt addsimps @{thms   Let_def}
+            (* delsimps @{thms binarysearch.simps blas.simps} *)
+          val f = Context_Rules.add Classical.safe_intro Classical.unsafe_intro Context_Rules.intro_query
+  
+        
+          fun string_of_thms ctxt args =
+            Pretty.string_of (Proof_Context.pretty_fact ctxt ("", Attrib.eval_thms ctxt args));
+   
+  
+          val Const ("Transpile.refines", _) $ L $ R  = goal_t_bool 
+  
+          val Const (te2_str, _) = te2 
+          
+          val _ = tracing "wee"
+          val ee = hd ( Proof_Context.get_thms ctxt (te2_str^".raw_induct"))
+
+          val Const (te_str, _) = te 
+          val f'_simps = ( Proof_Context.get_thms ctxt (te_str^".simps"))
+
+          val _ = tracing (Thm.string_of_thm ctxt ee)
+          
+          val ee_vars = rev (Term.add_vars (Thm.full_prop_of ee) [])
+          val _ = map (fn (_,ty) => tracing (Syntax.string_of_typ ctxt ty)) ee_vars
+          
+          val ggg = (if length ee_vars = 6 
+            then
+              let 
+                val _ = tracing "TUPLED"
+                val ff = foldl1 HOLogic.mk_prod varsb 
+          
+                val _ = tracing (Syntax.string_of_term ctxt ff)
+          
+                val gg = infer_instantiate' ctxt  [NONE,SOME (Thm.cterm_of ctxt ff)] ee 
+                val _ = tracing (Thm.string_of_thm ctxt gg)
+                val ggg = asm_full_simplify 
+    (put_simpset HOL_ss ctxt 
+      addsimps @{thms prod.case}) gg
+                val _ = tracing (Thm.string_of_thm ctxt ggg)
+              in ggg end
+            else 
+              let
+                val _ = tracing "not TUPLED"
+                val insts = map (SOME o Thm.cterm_of ctxt) varsb
+                val gg = infer_instantiate' ctxt  (NONE :: insts) ee 
+              in
+                 gg
+              end)
+            val gggg = infer_instantiate' ctxt  [SOME (Thm.cterm_of ctxt insta)] ggg 
+   
+            val _ = tracing ("yip" ^ Thm.string_of_thm ctxt gggg)
+  
+  
+            fun tac ctxt =  (HEADGOAL (myprint_tac ctxt "AA"
+          THEN' resolve_tac ctxt @{thms refinesI}
+  THEN' myprint_tac ctxt "AB" THEN' simp_tac ctxt
+  THEN' myprint_tac ctxt "AC"
+          THEN' resolve_tac ctxt [gggg]
+  THEN' myprint_tac ctxt "AD" )) THEN print_tac ctxt "all" THEN
+            asm_full_simp_tac ctxt 2
+          THEN eresolve_tac ctxt (@{thms refinesD1[OF _ , rotated]} @ [asm_rl]) 1
+          THEN (HEADGOAL ( EqSubst.eqsubst_tac ctxt [0] f'_simps
+                THEN' myprint_tac ctxt "aaae"
+                 THEN'  REPEAT_DETERM' ( FIRST' [ resolve_tac ctxt transpile_rules,
+                 resolve_tac ctxt @{thms refinesI} THEN' Method.assm_tac ctxt]
+                       THEN' myprint_tac ctxt "ae" )))
+  
+          val thm = Goal.prove_internal ctxt [] goal (fn _ => tac ctxt) 
+   
+          val thm = singleton (Variable.export ctxt ctxt_orig) thm
+   
+          val  Const (fun_name, fun_ty) = te
+          val defname = Binding.name fun_name
+  
+          val _ = tracing ("UNDER"^Syntax.string_of_term ctxt te)
+          val (_, ctxt) = Local_Theory.note (
+            (Binding.qualify_name true defname "correct_translate", @{attributes [transpile_rules]}),
+            [thm]
+          ) ctxt_orig 
+        in
+          ctxt
+        end
+  
+       val ctxt = prove_goal ctxt goal_t  
+      in  
+        ctxt
+      end
+
+    fun via_fun u = let 
+        val goal = goal_t 
+        val ctxt_orig = ctxt
+        val (goal, ctxt) = yield_singleton (Variable.import_terms true) goal ctxt
+        val _ = tracing (Syntax.string_of_term ctxt goal)
+        val Const ("HOL.Trueprop", _) $ goal_t_bool = goal 
+        val goal_t = goal 
+        val _ = tracing ("GoAL:"^Syntax.string_of_term ctxt goal_t)
+        val goal = goal |> Thm.cterm_of ctxt  
+        val rules = transpile_rules |> Tactic.build_net
+   
+  
+        val aee = (case Function_Common.import_function_data te2 ctxt of
+                  SOME info => info
+                | NONE => error ("Not a function: " ^ quote (Syntax.string_of_term ctxt te2)))
+        
+      
+        val { termination, fs, R, add_simps, case_names, psimps,
+          pinducts, defname, fnames, cases, dom, pelims, simps, inducts,  ...} = aee
+    
+        val simp = (case simps of NONE => error ("Simp rule not available!")
+                  | SOME simps => simps)
+        val inducts = (case inducts of NONE => error ("Simp rule not available!")
+                  | SOME inducts => inducts)
+     
+     
+  
+        val Const (te2_str, _) = te2  
+        val f_simps = ( Proof_Context.get_thms ctxt (te2_str^".simps"))
+    
+        val induction_rule = Function.get_info ctxt te2 |> #inducts |> the
+        val f'_simps = Function.get_info ctxt te |> #simps |> the
+                         
+
+        fun mk_effect ctxt =
+          let  
+            val ef = @{mk_term "refines ?psc ?ppsc"}
+            val (_, ctxt) = yield_singleton (Variable.import_terms true) ef ctxt
+            
+            val nctxt = Variable.names_of ctxt    
+            val vars = Name.invent nctxt "" 1 
+            val vars_n = map Var ((map (fn x => (x,0)) vars) ~~ [natT])
+            
+            val _ = tracing ("AA "  ^ (Syntax.string_of_term ctxt ef))
+            val tea = fold_rev lambda (varsb  ) ef
+            val _ = tracing ("C "  ^ (Syntax.string_of_term ctxt tea))
+          in tea end
+
+        val _ = tracing (Thm.string_of_thm ctxt (hd induction_rule))
+        val insta = mk_effect ctxt
+        val insta_ir =  infer_instantiate' ctxt  [SOME (Thm.cterm_of ctxt insta)] (hd induction_rule) 
+   
+        val _ = tracing ("yip" ^ Thm.string_of_thm ctxt insta_ir)
+        val _ = tracing "f_simps"
+        val _ = map (fn thm => tracing (Thm.string_of_thm ctxt thm)) f'_simps
+        
+        val _ = tracing ("WHAT")
+    
+        fun tac ctxt =  (ALLGOALS (myprint_tac ctxt ""
+          THEN' resolve_tac ctxt [insta_ir]
+          THEN_ALL_NEW ( myprint_tac ctxt "there1"  (* why is this executed twice ? *)
+            THEN' (EqSubst.eqsubst_tac ctxt [0] f_simps  )
+            THEN' myprint_tac ctxt "there2"
+            THEN' (EqSubst.eqsubst_tac ctxt [0] f'_simps 
+            THEN' myprint_tac ctxt "there3"
+            THEN' REPEAT_DETERM' (CHANGED o (
+                     FIRST' [resolve_tac ctxt transpile_rules,
+                              Method.assm_tac ctxt  ] )
+          ))))) 
+    
+        val thm = Goal.prove_internal ctxt [] goal (fn _ => tac ctxt) 
+     
+        val thm = singleton (Variable.export ctxt ctxt_orig) thm
+    
+        val defname =  Function_Common.import_function_data te ctxt
+              |> the |> #defname
+    
+        val _ = tracing ("UNDER"^Syntax.string_of_term ctxt te)
+        val (_, ctxt) = Local_Theory.note (
+          (Binding.qualify_name true defname "correct_translate", @{attributes [transpile_rules]}),
+          [thm]
+        ) ctxt_orig   
+      in
+        ctxt
+      end
+
+
+    fun via_def u = let
+        val _ = ()
+        val Const (te_str, _) = te  
+        val f'_flattens = ( Proof_Context.get_thms ctxt (te_str^".flattens"))
+        val [f'_def] = ( Proof_Context.get_thms ctxt (te_str^"_def")) 
+        val _ =  tracing (Thm.string_of_thm ctxt f'_def) 
+        val folded_r_thms = map (Local_Defs.fold ctxt [f'_def]) f'_flattens
+        val _ = map (fn th => tracing (Thm.string_of_thm ctxt th)) folded_r_thms
+        val Const (fun_name, fun_ty) = te
+        val defname = Binding.name fun_name
+        val (_, ctxt) = Local_Theory.note (
+          (Binding.qualify_name true defname "correct_translate", @{attributes [transpile_rules]}),
+          folded_r_thms
+        ) ctxt  
+      in
+        ctxt
+      end
+
+
+    val ctxt = (case old_info of NONE => 
+          (if defined_by_partial_function ctxt te then via_part_fun te te2 varsb
+            else via_def ())
+        | SOME old_info => via_fun ())  
+
+    
+  in ctxt
+end
+
+
+fun transpile_prove_cmd (binding1, binding2) lthy =
+  let 
+    val _ = tracing "transpile_prove"
+    val ctxt =  mkk2 binding1 binding2 lthy 
+  in
+    ctxt
+  end
+
+val transpile_prove_parser = Parse.term -- Parse.term 
+
+val _ =
+  Outer_Syntax.local_theory @{command_keyword transpile_prove}
+  "Define a new ground constant from an existing function definition"
+    (transpile_prove_parser >> transpile_prove_cmd)
+
+\<close>
+
+
+subsection \<open>Setup \<close>
+
+
+
+  lemma HTM_heap_fixp_codegen:
+    assumes DEF: "f \<equiv> Heap_Monad.heap.fixp_fun cB"
+    assumes M: "(\<And>x. Heap_Monad.mono_Heap (\<lambda>f. cB f x))"
+    shows "f x = cB f x"
+    unfolding DEF
+    apply (rule fun_cong[of _ _ x])
+    apply (rule Heap_Monad.heap.mono_body_fixp)
+    apply fact
+    done
+
+
+  ML \<open>
+    structure Sepref_Extraction = struct
+      val heap_extraction: Refine_Automation.extraction = {
+          pattern = Logic.varify_global @{term "Heap_Monad.heap.fixp_fun x"},
+          gen_thm = @{thm HTM_heap_fixp_codegen},
+          gen_tac = (fn ctxt => 
+            Pf_Mono_Prover.mono_tac ctxt
+          )
+        }
+
+      val setup = I 
+        (*#> Refine_Automation.add_extraction "trivial" triv_extraction*)
+        #> Refine_Automation.add_extraction "heap" heap_extraction
+
+    end
+    \<close>
+
+setup Sepref_Extraction.setup 
 
 
 
