SepLogicTime/Transpile_Tests.thy
@@ -1,0 +1,529 @@
+theory Transpile_Tests
+  imports Transpile BinarySearch_Impl RBTree_Impl Skew_Heap_Impl DynamicArray2 
+      "SeprefTime.Remdups" "SeprefTime.Kruskal_Time"
+  MergeSort_Impl
+
+   "HOL-Library.Code_Target_Numeral"
+begin
+
+section \<open>Transpilation by hand -- an example\<close>
+
+schematic_goal p: "refines ?G (binarysearch l r x a)"   
+  apply(subst binarysearch.simps)
+  apply(rule transpile_rules refines_flatten)+ done
+
+partial_function (heap) aahh where
+"aahh l r x a = (if r \<le> l then Heap_Monad.return False
+  else if r \<le> l + 1 then Array.nth a l \<bind> (\<lambda>v. Heap_Monad.return (v = x))
+       else let b = avg l r
+            in Array.nth a b \<bind>
+               (\<lambda>c. if c = x then Heap_Monad.return True
+                    else if c < x then aahh (b + 1) r x a else aahh l b x a))"
+
+lemma refines_binarysearch: "refines (aahh l r x a) (binarysearch l r x a)"
+  unfolding refines_def
+proof safe
+  fix h h' ra n
+  assume *: "Heap_Time_Monad.effect (binarysearch l r x a) h h' ra n"
+  
+  note f =  binarysearch.raw_induct[where P="\<lambda>l r x a h h' ra n. Heap_Monad.effect (aahh l r x a) h h' ra", where xa="(((l,r),x),a)", simplified]
+
+  show "Heap_Monad.effect (aahh l r x a) h h' ra" 
+  proof (rule f[OF _ *], goal_cases) 
+    case (1 f l r x a la ra xa aa)
+    from 1(1) have IH: "\<And>l r x a. refines (aahh l r x a) (f l r x a) " unfolding refines_def by auto 
+    show ?case apply(rule refinesD1[OF _ 1(2)])
+      apply(subst aahh.simps)
+      apply(rule transpile_rules IH)+
+      done
+  qed
+qed
+
+
+thm refines_HT'[OF _ refines_binarysearch]
+
+
+lemma flatten_correct: "sorted xs \<Longrightarrow> r \<le> length xs \<Longrightarrow> l \<le> r \<Longrightarrow>
+   <a \<mapsto>\<^sub>a xs > aahh l r x a
+       <\<lambda>ra. a \<mapsto>\<^sub>a xs * \<up> (ra = (\<exists>i\<ge>l. i < r \<and> xs ! i = x))>\<^sub>t"
+  apply(rule refines_HT) 
+     apply(rule refines_binarysearch)
+    apply(rule binarysearch_correct')
+      apply simp
+     apply simp
+    apply simp
+   apply (simp add: forget_it)
+  apply(rule ext) apply (simp add: forget_it)
+  done
+
+
+section "Example -- MergeSort"
+
+
+thm mergeSort_correct
+ 
+transpile_define atake': atake_def
+transpile_prove atake' atake
+
+
+transpile_define adrop': adrop_def
+transpile_prove adrop' adrop
+
+transpile_define mergeinto': mergeinto.simps
+transpile_replay mergeinto' mergeinto
+transpile_prove mergeinto' mergeinto
+
+transpile_define merge_sort_impl': merge_sort_impl.simps
+transpile_prove merge_sort_impl' merge_sort_impl
+print_theorems
+
+thm prod.case
+
+lemma merge_sort_impl'_correct:
+  "<p \<mapsto>\<^sub>a xs> merge_sort_impl' p <\<lambda>_. p \<mapsto>\<^sub>a sort xs>\<^sub>t" 
+  apply(rule refines_HT) 
+     apply(rule Transpile_Tests.merge_sort_impl'.correct_translate)
+    apply(rule mergeSort_correct) 
+   apply (simp add: forget_it) 
+  apply (simp add: forget_it)
+  done
+
+
+section \<open>Example -- Dynamic Array\<close>
+
+lemma [transpile_rules]: "(\<And>al ar. refines (f' al ar) (f al ar)) \<Longrightarrow>
+    refines (case x  of  Dyn_Array al ar \<Rightarrow> f' al ar) (case x  of  Dyn_Array al ar \<Rightarrow> f al ar)" 
+  by(auto split: dynamic_array.splits)
+
+
+
+transpile_define array_copy': array_copy.simps
+transpile_replay array_copy' array_copy
+transpile_prove array_copy' array_copy 
+
+transpile_define push_array': push_array_def[unfolded array_max_def array_length_def
+                                              push_array_basic_def double_length_def]
+transpile_prove push_array' push_array
+
+transpile_define dfilter_aux': dfilter_aux.simps
+transpile_replay dfilter_aux' dfilter_aux
+transpile_prove dfilter_aux' dfilter_aux
+
+
+text \<open>an alternative way to synthesize\<close>
+experiment
+begin
+schematic_goal refines_dyn_array_new:  "refines ?G dyn_array_new"
+  unfolding dyn_array_new_def 
+  apply(rule transpile_rules )+ 
+    done
+concrete_definition dyn_array_new'  uses refines_dyn_array_new is "refines ?G dyn_array_new"
+print_theorems
+lemmas [transpile_rules] = dyn_array_new'.refine
+end
+
+transpile_define dyn_array_new': dyn_array_new_def
+transpile_prove dyn_array_new' dyn_array_new
+
+transpile_define dfilter_impl': dfilter_impl_def
+transpile_prove dfilter_impl' dfilter_impl
+print_theorems
+
+lemma "<a \<mapsto>\<^sub>a xs> dfilter_impl' a P
+       <\<lambda>r. a \<mapsto>\<^sub>a xs * forget (dyn_array (filter P xs) r)>\<^sub>t"
+  apply(rule refines_HT) 
+     apply(rule Transpile_Tests.dfilter_impl'.correct_translate)
+    apply(rule dfilter_impl_rule) 
+   apply (simp add: forget_it) 
+  apply (simp add: forget_it)
+  done
+
+export_code dfilter_impl' in SML
+
+
+transpile_define destroy': destroy_def
+transpile_prove destroy' destroy
+
+
+subsection \<open>Example -- binarysearch\<close>
+
+transpile_define   binarysearch': binarysearch.simps
+transpile_prove binarysearch' binarysearch
+
+lemma binarysearch'_HT: "sorted xs \<Longrightarrow> r \<le> length xs \<Longrightarrow> l \<le> r \<Longrightarrow>
+   <a \<mapsto>\<^sub>a xs > binarysearch' l r x a
+       <\<lambda>ra. a \<mapsto>\<^sub>a xs * \<up> (ra = (\<exists>i\<ge>l. i < r \<and> xs ! i = x))>\<^sub>t"
+  apply(rule refines_HT) 
+     apply(rule Transpile_Tests.binarysearch'.correct_translate)
+    apply(rule binarysearch_correct')
+      apply (simp_all  add: forget_it) 
+  done
+
+
+section "Example -- Red Black Tree"
+
+fun rbt_btree :: "('a::heap, 'b::heap) rbt \<Rightarrow> ('a, 'b) rbt_node ref option \<Rightarrow> Assertions.assn" where
+  "rbt_btree Leaf p = \<up>(p = None)"
+| "rbt_btree (rbt.Node lt c k v rt) (Some p) = (\<exists>\<^sub>Alp rp. p \<mapsto>\<^sub>r Node lp c k v rp * rbt_btree lt lp * rbt_btree rt rp)"
+| "rbt_btree (rbt.Node lt c k v rt) None = false"
+
+lemma forget_rbt_btree[forget_it]: "forget (RBTree_Impl.btree t p) = rbt_btree t p"
+  apply(induction t arbitrary: p) apply (auto simp: forget_it)
+  subgoal for t1 x2 x3 x4 t2 p apply (cases p) apply (auto simp: forget_it)
+    done
+  done
+
+schematic_goal forget_rbt_map_assn: "forget (rbt_map_assn M b) = ?G"
+  unfolding rbt_map_assn_def
+  apply(subst forget_it)+
+  by(rule refl)
+concrete_definition rbt_map_assn_flat uses forget_rbt_map_assn
+lemmas [forget_it] = rbt_map_assn_flat.refine
+thm rbt_map_assn_flat_def
+
+transpile_define get_color': get_color_def
+transpile_prove get_color' get_color
+
+transpile_define set_color': set_color_def
+transpile_prove set_color' set_color
+
+transpile_define btree_rotate_r': btree_rotate_r_def
+transpile_prove btree_rotate_r' btree_rotate_r
+
+transpile_define btree_rotate_l': btree_rotate_l_def
+transpile_prove btree_rotate_l' btree_rotate_l 
+
+transpile_define btree_balanceR': btree_balanceR_def
+transpile_prove btree_balanceR' btree_balanceR 
+
+transpile_define btree_balance': btree_balance_def
+transpile_prove btree_balance' btree_balance
+ 
+
+transpile_define btree_constr': btree_constr_def
+transpile_prove btree_constr' btree_constr 
+
+transpile_define rbt_ins': rbt_ins.simps
+transpile_prove rbt_ins' rbt_ins
+
+transpile_define rbt_paint': RBTree_Impl.paint_def
+transpile_prove rbt_paint' RBTree_Impl.paint
+
+transpile_define rbt_insert': rbt_insert_def
+transpile_prove rbt_insert' rbt_insert 
+
+lemma rbt_insert'_HT:  "<rbt_map_assn_flat M b> 
+      rbt_insert' k v b
+     <rbt_map_assn_flat (M {k \<rightarrow> v})>\<^sub>t"
+  apply(rule refines_HT) 
+     apply(rule Transpile_Tests.rbt_insert'.correct_translate)
+    apply(rule rbt_insert_rule)
+      apply (simp add: forget_it)
+      apply (simp add: forget_it) 
+  done
+
+transpile_define rbt_search': rbt_search.simps
+transpile_prove rbt_search' rbt_search
+
+lemma rbt_search'_HT:  "<rbt_map_assn_flat M b> 
+     rbt_search' x b
+     <\<lambda>r. rbt_map_assn_flat M b * pure_assn(r = M\<langle>x\<rangle>)>\<^sub>t"
+  (* oddity: using \<up> syntax does lead to exceptoion:
+     exception COERCION_GEN_ERROR fn raised (line 678 of "~~/src/Tools/subtyping.ML") *)
+  apply(rule refines_HT) 
+     apply(rule Transpile_Tests.rbt_search'.correct_translate)
+    apply(rule rbt_search)
+      apply (simp add: forget_it)
+      apply (simp add: forget_it) 
+  done 
+
+transpile_define btree_balR': btree_balR_def
+transpile_prove btree_balR' btree_balR
+
+transpile_define btree_balL': btree_balL_def
+transpile_prove btree_balL' btree_balL
+
+transpile_define btree_combine': btree_combine.simps
+transpile_prove btree_combine' btree_combine 
+
+transpile_define rbt_del': rbt_del.simps
+transpile_prove rbt_del' rbt_del
+
+transpile_define rbt_delete': rbt_delete_def
+transpile_prove rbt_delete' rbt_delete
+
+lemma rbt_delete'_HT:  "<rbt_map_assn_flat M b> 
+     rbt_delete' k b
+     <rbt_map_assn_flat (delete_map k M)>\<^sub>t"
+  apply(rule refines_HT) 
+     apply(rule Transpile_Tests.rbt_delete'.correct_translate)
+    apply(rule rbt_delete_rule)
+      apply (simp add: forget_it)
+      apply (simp add: forget_it) 
+  done
+
+transpile_define rbt_empty': RBTree_Impl.tree_empty_def
+transpile_prove rbt_empty' RBTree_Impl.tree_empty 
+ 
+theorem rbt_empty'_rule:
+  "<emp> rbt_empty' <rbt_map_assn_flat empty_map>"
+  apply(rule refines_HT) 
+     apply(rule Transpile_Tests.rbt_empty'.correct_translate)
+    apply(rule rbt_empty_rule)
+      apply (simp add: forget_it)
+      apply (simp add: forget_it) 
+  done
+
+
+definition "rbt_empty_int_set == rbt_empty' :: (int, unit) rbt_node ref option Heap"
+definition "rbt_insert_int_set k b \<equiv> rbt_insert' (k::int) () b"
+definition "rbt_search_int_set \<equiv> rbt_search' :: int  \<Rightarrow> (int, unit) btree \<Rightarrow> unit option Heap" 
+definition "rbt_delete_int_set \<equiv> rbt_delete' :: int  \<Rightarrow> (int, unit) btree \<Rightarrow> (int, unit) btree Heap_Monad.Heap "
+
+export_code integer_of_int int_of_integer 
+  rbt_empty_int_set rbt_insert_int_set rbt_search_int_set rbt_delete_int_set
+  in SML module_name RBT
+
+ 
+section "Example -- Skew Heap" 
+fun btree_flat :: "'a::heap tree \<Rightarrow> 'a node ref option \<Rightarrow> Assertions.assn" where
+  "btree_flat Tree.Leaf p = \<up>(p = None)"
+| "btree_flat \<langle>lt, v, rt\<rangle> (Some p) = (\<exists>\<^sub>Alp rp. p \<mapsto>\<^sub>r Tree_Impl.Node lp v rp * btree_flat lt lp * btree_flat rt rp)"
+| "btree_flat \<langle>lt, v, rt\<rangle> None = false"
+
+lemma forget_btree: "forget (Tree_Impl.btree t p) = (btree_flat t p)"
+  apply(induct t arbitrary: p) apply (auto simp: forget_it)
+  subgoal for t1 x2 t2 p apply(cases p)  by (auto simp: forget_it) 
+  done
+ 
+
+schematic_goal forget_skew_heap_mset: "forget (skew_heap_mset T b) = ?G"
+  unfolding skew_heap_mset_def skew_heap_def
+  apply (subst forget_it forget_btree)+
+  by (rule refl)
+concrete_definition skew_heap_mset_flat uses forget_skew_heap_mset
+print_theorems
+lemmas [forget_it] =  skew_heap_mset_flat.refine 
+
+transpile_define skew_heap_merge_impl': merge_impl.simps
+transpile_prove skew_heap_merge_impl' merge_impl
+
+lemma skew_heap_merge'_rule:
+  "<skew_heap_mset_flat S a * skew_heap_mset_flat T b>
+    skew_heap_merge_impl' a b
+   <skew_heap_mset_flat (S + T)>\<^sub>t"
+  apply(rule refines_HT) 
+     apply(rule Transpile_Tests.skew_heap_merge_impl'.correct_translate)
+    apply(rule skew_heap_merge_rule)
+   apply (simp add: forget_it) 
+  apply (simp add: forget_it) 
+  done
+
+transpile_define skew_heap_constr': skew_heap_constr_def[unfolded tree_constr_def]
+transpile_prove skew_heap_constr' skew_heap_constr 
+
+
+transpile_define skew_heap_insert_impl': insert_impl_def
+transpile_prove skew_heap_insert_impl'  insert_impl  
+ 
+lemma skew_heap_insert_impl'_rule:
+  "<skew_heap_mset_flat S a >
+    skew_heap_insert_impl' x a
+   <skew_heap_mset_flat ({#x#} + S)>\<^sub>t"
+  apply(rule refines_HT) 
+     apply(rule Transpile_Tests.skew_heap_insert_impl'.correct_translate)
+    apply(rule skew_heap_insert_rule)
+      apply (simp add: forget_it)
+      apply (simp add: forget_it) 
+  done
+
+transpile_define skew_heap_del_min_impl': del_min_impl.simps
+transpile_prove skew_heap_del_min_impl' del_min_impl
+
+lemma skew_heap_del_min_rule'_rule:
+  "S \<noteq> {#} \<Longrightarrow><skew_heap_mset_flat S a>
+    skew_heap_del_min_impl'  a
+   <skew_heap_mset_flat (S - {# Min_mset S #}) >\<^sub>t"
+  apply(rule refines_HT) 
+     apply(rule Transpile_Tests.skew_heap_del_min_impl'.correct_translate)
+    apply(rule skew_heap_del_min_rule)
+    apply simp
+   apply (simp add: forget_it)
+  apply (simp add: forget_it) 
+  done
+
+term skew_heap_empty
+thm skew_heap_empty_rule''
+
+
+transpile_define skew_heap_empty': skew_heap_empty_def[unfolded Tree_Impl.tree_empty_def]
+transpile_prove skew_heap_empty' skew_heap_empty  
+
+lemma "<emp> skew_heap_empty' <skew_heap_mset_flat {#}>\<^sub>t"
+  apply(rule refines_HT) 
+     apply(rule Transpile_Tests.skew_heap_empty'.correct_translate)
+    apply(rule skew_heap_empty_rule'') 
+   apply (simp add: forget_it)
+  apply (simp add: forget_it) 
+  done
+
+export_code skew_heap_empty' skew_heap_insert_impl'
+          skew_heap_del_min_impl' skew_heap_insert_impl' in SML
+
+section "Examples -- with fixp combinator"
+
+
+subsection \<open>Remove Duplicates\<close>
+
+lemma [transpile_rules]:   "refines (return v) (ureturn v)"
+  unfolding refines_def return_def ureturn_def
+    Heap_Time_Monad.effect_def Heap_Monad.effect_def
+    Heap_Time_Monad.heap_def Heap_Monad.heap_def
+  by auto
+
+lemma [transpile_rules]:   "
+  (\<And>a b. refines (f' a b) (f a b)) \<Longrightarrow>
+  refines (case x of (a,b) \<Rightarrow> f' a b) (case x of (a,b) \<Rightarrow> f a b)"
+  by (auto split: prod.splits)
+
+transpile_define set_empty': set_empty_def
+transpile_prove set_empty' set_empty
+
+transpile_define rbt_mem': rbt_mem_def
+transpile_prove rbt_mem' rbt_mem
+
+transpile_define rbt_set_insert': rbt_set_insert_def
+transpile_prove rbt_set_insert' rbt_set_insert
+
+transpile_define remdups_impl': remdups_impl_def[unfolded heap_WHILET_def, THEN meta_eq_to_obj_eq]
+transpile_prove  remdups_impl' remdups_impl
+print_theorems
+
+lemmas [code del] = remdups_impl'_def
+thm remdups_impl'_def[unfolded to_meta_eq, unfolded   ]
+prepare_code_thms remdups_impl'_def[unfolded to_meta_eq, unfolded   ]
+ 
+definition remdups_impl'_nat :: "nat list \<Rightarrow> nat dynamic_array Heap_Monad.Heap" where
+  "remdups_impl'_nat as \<equiv>remdups_impl' as"                 
+prepare_code_thms remdups_impl'_nat_def[unfolded remdups_impl'_def]
+ 
+export_code remdups_impl'_nat in SML module_name REMDUPS
+
+
+subsection \<open>Kruskal\<close>
+
+
+term kruskal'
+thm kruskal'_def
+
+term kruskal_final
+thm kruskal_final_def
+
+thm Kruskal_Time.Kruskal_final.E
+
+term Kruskal_intermediate_Impl.kruskal
+
+
+lemma list_case_reines[transpile_rules]:
+    "refines f' f 
+    \<Longrightarrow> (\<And>x xs. refines (g' x xs) (g x xs))
+    \<Longrightarrow>  refines (case x of [] \<Rightarrow> f' | (x#xs) \<Rightarrow> g' x xs)
+         (case x of [] \<Rightarrow> f | (x#xs) \<Rightarrow> g x xs)"
+  by (auto split: list.splits)
+
+
+
+lemma case_wrap_refine[transpile_rules]:
+  "(\<And>a. refines (f' a) (f a)) \<Longrightarrow> refines (case_wrap f' x) (case_wrap f x)"
+  by(auto split: wrap.splits)
+
+transpile_define maxn'': maxn'.simps
+transpile_replay maxn'' maxn'
+transpile_prove maxn'' maxn'
+
+transpile_define maxn': maxn_def
+transpile_prove maxn' maxn
+
+
+
+(*
+definition remdups_impl_wrap :: "wrap list \<Rightarrow> wrap dynamic_array Heap_Time_Monad.Heap" where
+  "remdups_impl_wrap as = remdups_impl as"  
+
+transpile_define remdups_impl_wrap': remdups_impl_wrap_def[unfolded remdups_impl_def heap_WHILET_def]
+transpile_prove remdups_impl_wrap' remdups_impl_wrap
+
+lemma [transpile_rules]: "refines (remdups_impl_wrap' as) (remdups_impl as)"
+  using Transpile_Tests.remdups_impl_wrap'.correct_translate  unfolding remdups_impl_wrap_def
+  by auto
+
+thm remdups_impl_wrap'_def[no_vars]
+*)
+
+thm kruskal'_def 
+term sortEdges'
+transpile_define sortEdges'': sortEdges'_def
+transpile_prove sortEdges'' sortEdges'
+
+thm uf_init_def
+transpile_define uf_init': uf_init_def[THEN meta_eq_to_obj_eq]
+transpile_prove uf_init' uf_init
+
+transpile_define uf_rep_of': uf_rep_of.simps
+transpile_prove uf_rep_of' uf_rep_of 
+
+transpile_define uf_compress': uf_compress.simps
+transpile_prove uf_compress' uf_compress 
+
+
+
+transpile_define uf_rep_of_c': uf_rep_of_c_def[THEN meta_eq_to_obj_eq]
+transpile_prove uf_rep_of_c' uf_rep_of_c
+
+transpile_define uf_cmp': uf_cmp_def[THEN meta_eq_to_obj_eq]
+transpile_prove uf_cmp' uf_cmp
+
+transpile_define uf_union' : uf_union_def[THEN meta_eq_to_obj_eq]
+transpile_prove uf_union' uf_union
+ 
+
+
+thm  kruskal_final_def[of getEdges_impl]
+definition "kruskal_final_final as = kruskal_final (Heap_Time_Monad.return as)"
+thm kruskal_final_final_def[unfolded kruskal_final_def kruskal'_def]
+transpile_define kruskal_final': kruskal_final_final_def[unfolded kruskal_final_def kruskal'_def]
+transpile_prove kruskal_final' kruskal_final
+
+thm kruskal_final'_def
+definition "Kruskal_fun as \<equiv> do { k \<leftarrow> kruskal_final' as; a \<leftarrow> destroy' k; Array.freeze a}"
+prepare_code_thms (in -) Kruskal_fun_def[unfolded kruskal_final'_def]
+print_theorems
+
+
+
+ 
+
+ 
+export_code integer_of_int int_of_integer
+    integer_of_nat  nat_of_integer
+    Kruskal_fun in SML module_name KRUSKAL
+ 
+ 
+
+section "partial_function strangeness"
+
+thm rbt_ins.raw_induct (* no tuple *)
+thm btree_combine.raw_induct (* no tuple *)
+thm binarysearch.raw_induct (* tuple *)
+thm rbt_search.raw_induct (* tuple *)
+thm rbt_del.raw_induct (* tuple *)
+
+partial_function (heap_time) rbt_del2 ::
+  "'a::{heap,linorder} \<Rightarrow> ('a, 'b::heap) btree \<Rightarrow> ('a, 'b) btree Heap_Time_Monad.Heap" where
+  "rbt_del2 x p = (case p of
+     None \<Rightarrow> Heap_Time_Monad.return None
+   | Some pp \<Rightarrow> do {
+      t \<leftarrow> !pp;rbt_del2 x (RBTree_Impl.lsub t)})"
+thm rbt_del2.raw_induct (* tuple *)
+
+end
